proof/eclib/CircuitBindings.ec
@@ -1,0 +1,808 @@
+(* ==================================================================== *)
+require import AllCore List Ring IntDiv BitEncoding.
+require import StdRing StdOrder QFABV.
+require import List_extra.
+
+from Jasmin require import JWord JArray.
+
+import BS2Int.
+
+require import JWordExtra.
+
+import BitChunking.
+
+(* ==================================================================== *)
+(* PAE: array-extras abstract theory (ported from mldsa JArrayExtra.ec).*)
+(* Embedded here so XArray* files get it transitively from              *)
+(* CircuitBindings rather than via a separate file.                     *)
+(* ==================================================================== *)
+abstract theory PAE.
+  op size : int.
+
+  clone import PolyArray as A with op size <- size.
+
+  (* -------------------------------------------------------------------- *)
+  op eqon ['a] (a1 a2 : 'a t) (base len : int) =
+    forall i, base <= i < base + len => a1.[i] = a2.[i].
+
+  (* -------------------------------------------------------------------- *)
+  op eqexcept ['a] (a1 a2 : 'a t) (base len : int) =
+    forall i, !(base <= i < base + len) => a1.[i] = a2.[i].
+
+  (* -------------------------------------------------------------------- *)
+  lemma fill_congr (f g : int -> 'a) (k1 k2 : int) (len1 len2 : int) (a1 a2 : 'a t) :
+       k1 = k2
+    => len1 = len2
+    => (forall i, k1 <= i < k1 + len1 => f i = g i)
+    => a1 = a2
+    => fill f k1 len1 a1 = fill g k2 len2 a2.
+  proof.
+  by move=> <<- <<- eq <<-; apply: ext_eq=> i rgi; rewrite !filliE //#.
+  qed.
+
+  (* -------------------------------------------------------------------- *)
+  lemma fill_eqexcept (f : int -> 'a) (k : int) (len : int) (a : 'a t) :
+    eqexcept (fill f k len a) a k len.
+  proof.
+  move=> i *; case: (0 <= i < size) => *; last by rewrite !get_out.
+  by rewrite filliE // ifF //#.
+  qed.
+
+  (* -------------------------------------------------------------------- *)
+  lemma fill_swap ['a] (f g : int -> 'a) (k1 k2 : int) (len1 len2 : int) (a : 'a t) :
+       k1 + len1 <= k2
+    => fill g k1 len1 (fill f k2 len2 a) = fill f k2 len2 (fill g k1 len1 a).
+  proof. by move=> *; apply/ext_eq=> i *; rewrite !filliE //#. qed.
+
+  (* -------------------------------------------------------------------- *)
+  op replace_ ['a] (a : 'a t) (base : int) (s : 'a list) =
+    fill (fun i => nth witness s (i - base)) base (size s) a.
+
+  (* -------------------------------------------------------------------- *)
+  lemma replace_nil ['a] (a : 'a t) (base : int) : replace_ a base [] = a.
+  proof. by apply/ext_eq=> i *; rewrite /replace_ filliE //= ifF //#. qed.
+
+  hint simplify replace_nil.
+
+  (* -------------------------------------------------------------------- *)
+  lemma replace_eqexcept (a : 'a t) (base : int) (s : 'a list) :
+    eqexcept (replace_ a base s) a base (size s).
+  proof. by apply: fill_eqexcept. qed.
+
+  (* -------------------------------------------------------------------- *)
+  lemma replace_mkseq ['a] (f : int -> 'a) (a : 'a t) (base len : int) :
+    replace_ a base (mkseq f len) = fill (fun i => f (i - base)) base len a.
+  proof.
+  apply/ext_eq=> i rgi @/replace_; rewrite !filliE //=.
+  rewrite size_mkseq; case: (len < 0) => [lt0_len|/lezNgt gt0_len].
+  - by rewrite !ifF //#.
+  rewrite lez_maxr //; case: (base <= i < base + len) => // ?.
+  by rewrite nth_mkseq 1:/#.
+  qed.
+
+  (* -------------------------------------------------------------------- *)
+  lemma replace_swap ['a] (a : 'a t) (b1 b2 : int) (s1 s2 : 'a list) :
+       b1 + size s1 <= b2
+    => replace_ (replace_ a b2 s2) b1 s1 = replace_ (replace_ a b1 s1) b2 s2.
+  proof. by move=> * @/replace_; rewrite fill_swap. qed.
+
+  (* -------------------------------------------------------------------- *)
+  lemma replaceC ['a] (a : 'a t) (b1 b2 : int) (s1 s2 : 'a list) :
+       b1 + size s1 <= b2 \/ b2 + size s2 <= b1
+    => replace_ (replace_ a b2 s2) b1 s1 = replace_ (replace_ a b1 s1) b2 s2.
+  proof.
+  case (b1 + size s1 <= b2) => [/replace_swap ->//|].
+  case (b2 + size s2 <= b1) => [/replace_swap ->//|].
+  done.
+  qed.
+
+  (* -------------------------------------------------------------------- *)
+  lemma replace_cat ['a] (a : 'a t) (base : int) (s1 s2 : 'a list) :
+    replace_ a base (s1 ++ s2) = replace_ (replace_ a base s1) (base + size s1) s2.
+  proof.
+  apply/ext_eq=> i *; rewrite /replace_ !filliE //=.
+  by rewrite size_cat nth_cat /=; smt(size_ge0).
+  qed.
+end PAE.
+
+(* ==================================================================== *)
+theory T.
+op bool2bits (b : bool) : bool list = [b].
+op bits2bool (b: bool list) : bool = List.nth false b 0.
+
+op i2b (i : int) = (i %% 2 <> 0).
+op b2si (b : bool) = 0.
+
+bind bitstring bool2bits bits2bool b2i b2si i2b bool 1.
+
+realize gt0_size    by done.
+realize size_tolist by done.
+realize tolistP     by done.
+realize tosintP     by done.
+realize oflistP     by smt(size_eq1).
+
+realize ofintP.
+proof.
+move=> i @/bits2bool @/int2bs.
+by rewrite (nth_mkseq false). 
+qed.
+
+realize touintP.
+proof.
+move=> b @/bool2bits.
+by rewrite bs2int_cons bs2int_nil.
+qed.
+end T.
+
+bind op bool (/\) "and".
+realize bvandP by move=> * @/bool2bits /#.
+
+bind op bool (\/) "or".
+realize bvorP by move=> * @/bool2bits /#.
+
+bind op bool Bool.(^^) "xor".
+realize bvxorP by move=> * @/bool2bits /#.
+
+(* ==================================================================== *)
+abstract theory BSBW.
+  op size : int.
+
+  clone import BitWord as BW with op size <- size.
+  clone import WE as WE with op size <- size, theory W <- BW.
+
+  op rol (w1 w2 : BW.t) = w1 `|<<<|` to_uint w2.
+  op ror (w1 w2 : BW.t) = w1 `|>>>|` to_uint w2.
+
+  op sar (w1 w2 : BW.t) : BW.t = w1 `|>>>` BW.to_uint w2.
+  op shr (w1 w2 : BW.t) : BW.t = w1  `>>>` BW.to_uint w2.
+  op shl (w1 w2 : BW.t) : BW.t = w1  `<<<` BW.to_uint w2.
+
+  bind bitstring BW.w2bits BW.bits2w BW.to_uint BW.to_sint BW.of_int BW.t size.
+
+  realize gt0_size    by done.
+  realize size_tolist by done.
+  realize tolistP     by exact: BW.w2bitsK.
+  realize oflistP     by exact: BW.bits2wK.
+  realize touintP     by move=> @/to_uint.
+
+  realize tosintP.
+  proof.
+  have ? := gt0_size; move=> w; apply/implyNb=> sz_ne1 /=.
+  by rewrite /msb -get_bits2w 1:/# w2bitsK -msbE /#.
+  qed.
+
+  realize ofintP.
+  proof. by move=> i @/of_int; rewrite int2bs_mod. qed.
+
+  bind op BW.t BW.( + ) "add".
+  realize bvaddP by exact BW.to_uintD.
+
+  bind op BW.t BW.([-]) "opp".
+  realize bvoppP by exact BW.to_uintN.
+
+  bind op BW.t BW.( * ) "mul".
+  realize bvmulP by exact BW.to_uintM.
+
+  bind op BW.t BW.(\udiv) "udiv".
+  realize bvudivP by exact WE.to_uintUD.
+
+  bind op BW.t BW.(\umod) "urem".
+  realize bvuremP by exact WE.to_uintUM.
+
+  bind op BW.t BW.andw "and".
+  realize bvandP.
+  proof.
+  by move=> w1 w2; rewrite /w2bits zip_map /= zipss -!map_comp.
+  qed.
+
+  bind op BW.t BW.orw "or".
+  realize bvorP.
+  proof.
+  by move=> w1 w2; rewrite /w2bits zip_map /= zipss -!map_comp.
+  qed.
+
+  bind op BW.t BW.(+^) "xor".
+  realize bvxorP.
+  proof.
+  by move=> w1 w2; rewrite /w2bits zip_map /= zipss -!map_comp.
+  qed.
+
+  bind op BW.t BW.invw "not".
+  realize bvnotP.
+  proof.
+  by move=> w; rewrite /invw /= eq_sym map_w2bits_w2bits.
+  qed.
+
+  bind op [BW.t] rol "rol".
+  realize bvrolP.
+  proof.
+  by move=> w1 w2 i ?; rewrite !get_w2bits /rol initE ifT.
+  qed.
+
+  bind op [BW.t] ror "ror".
+  realize bvrorP.
+  proof.
+  by move=> w1 w2 i ?; rewrite !get_w2bits /ror initE ifT.
+  qed.
+
+  bind op [BW.t] sar "ashr".
+  realize bvashrP.
+  proof. by move=> w1 w2; rewrite to_sint_sar // #smt:(to_uint_cmp). qed.
+
+  bind op [BW.t] shl "shl".
+  realize bvshlP.
+  proof. by move=> w1 w2; rewrite to_uint_shl // #smt:(to_uint_cmp). qed.
+
+  bind op [BW.t] shr "shr".
+  realize bvshrP.
+  proof. by move=> w1 w2; rewrite to_uint_shr // #smt:(to_uint_cmp). qed.
+
+  bind op [bool & BW.t] BW.(\ult) "ult".
+  realize bvultP by smt().
+
+  bind op [bool & BW.t] BW.(\ule) "ule".
+  realize bvuleP by smt().
+
+  bind op [bool & BW.t] BW.(\slt) "slt".
+  realize bvsltP by smt().
+
+  bind op [bool & BW.t] BW.(\sle) "sle".
+  realize bvsleP by smt().
+
+  (* FIXME: uniformize type parameter order for bindings *)
+  (* FIXME: uniformize binding treatment of booleans     *)
+  (* FIXME: here BSBW.size is required to be >= 1         *)
+  bind op [BW.t & bool] BW."_.[_]" "get".
+  realize bvgetP   by done.
+  realize eq1_size by done.
+  realize le_size  by smt(gt0_size).
+
+  bind op [bool & BW.t] BW.init "init".
+
+  realize size_1 by done.
+
+  realize bvinitP.
+  proof.
+  move=> f; rewrite init_bits2w bits2wK.
+  - by rewrite size_map size_iota.
+  - by rewrite flatten_mkseq_seq1.
+  qed.
+end BSBW.
+
+(* ==================================================================== *)
+clone BSBW as BSW8 with
+  op     size <- 8,
+  theory BW   <- W8  { rename "_XX" as "_8" },
+  theory WE   <- WE8.
+
+(* ==================================================================== *)
+abstract theory BSW.
+  op size : int.
+
+  clone import BitWordSH as W with op size <- size.
+
+  clone include BSBW with
+        op size <- size,
+    theory BW   <- W.
+
+  import WE.
+
+  bind op [W.t & W8.t] W.(`<<`) "shls".
+  realize bvshlsP.
+  proof. by move=> w1 w2; rewrite to_uint_shl // #smt:(W8.to_uint_cmp). qed.
+
+  bind op [W.t & W8.t] W.(`>>`) "shrs".
+  realize bvshrsP.
+  proof. by move=> w1 w2; rewrite to_uint_shr // #smt:(W8.to_uint_cmp). qed.
+
+  bind op [W.t & W8.t] W.(`|>>`) "ashrs".
+  realize bvashrsP.
+  proof. by move=> w1 w2; rewrite to_sint_sar // #smt:(W8.to_uint_cmp). qed.
+end BSW.
+
+(* ==================================================================== *)
+abstract theory BS_WB_WS_U.
+  op sizeS : int.
+  op sizeB : int.
+
+  axiom le_size : sizeS <= sizeB.
+
+  clone import BitWord as WS with
+    op size <- sizeS.
+
+  clone WE as WSE with
+        op size <- sizeS,
+    theory W    <- WS.
+
+  clone import BitWord as WB with
+    op size <- sizeB.
+
+  clone WE as WBE with
+        op size <- sizeB,
+    theory W    <- WB.
+
+  clone import BSBW as BSWS with 
+        op size <- sizeS,
+    theory BW   <- WS,
+    theory WE   <- WSE.
+
+  clone import BSBW as BSWB with 
+        op size <- sizeB,
+    theory BW   <- WB,
+    theory WE   <- WBE.
+
+  op truncateu'S (w : WB.t) : WS.t =
+    WS.of_int (WB.to_uint w).
+
+  op zeroextu'B (w : WS.t) : WB.t =
+    WB.of_int (WS.to_uint w).
+
+  op sigextu'B (w : WS.t) : WB.t =
+    WB.of_int (WS.to_sint w).
+
+  bind op [WB.t & WS.t] truncateu'S "truncate".
+
+  realize le_size by apply: le_size.
+
+  realize bvtruncateP.
+  proof.
+  move=> w @/truncateu'S @/w2bits; rewrite take_mkseq.
+  - by rewrite ge0_size le_size.
+  apply: eq_in_mkseq => i rgi /=; rewrite of_intwE rgi /=.
+  rewrite get_to_uint /int_bit /= modz_pow2_div 1:/#.
+  by rewrite modz_dvd -1:#smt:(le_size) (dvdz_exp2l _ 1) /#.
+  qed.
+
+  bind op [WS.t & WB.t] zeroextu'B "zextend".
+
+  realize le_size by apply: le_size.
+
+  realize bvzextendP.
+  proof.
+  have ? := WS.to_uint_cmp; move=> w @/zeroextu'B.
+  rewrite to_uintK_small //.
+  smt(WS.gt0_size le_size IntOrder.ler_weexpn2l).
+  qed.
+
+  bind op [WS.t & WB.t] sigextu'B "sextend".
+
+  realize le_size by apply: le_size.
+
+  realize bvsextendP.
+  proof.
+  move=> w @/sigextu'B; rewrite to_sintK_small //.
+  have [#] hlo hhi := WS.to_sint_cmp w.
+  smt(WS.gt0_size le_size IntOrder.ler_weexpn2l).
+  qed.
+end BS_WB_WS_U.
+
+(* ==================================================================== *)
+abstract theory BS_WB_WS.
+  op sizeS : int.
+  op sizeB : int.
+  op r     : int.
+
+  clone import BitWordSH as WS with
+    op size <- sizeS.
+
+  clone WE as WSE with
+        op size <- sizeS,
+    theory W    <- WS.
+
+  clone import BitWordSH as WB with
+    op size <- sizeB.
+
+  clone WE as WBE with
+        op size <- sizeB,
+    theory W    <- WB.
+  
+  clone import W_WS with
+        op sizeS <- sizeS, 
+        op sizeB <- sizeB,
+        op r     <- r,
+    theory WS    <- WS,
+    theory WB    <- WB.
+
+  clone import BSW as BSWS with 
+        op size <- sizeS,
+    theory W    <- WS,
+    theory WE   <- WSE.
+
+  clone import BSW as BSWB with 
+        op size <- sizeB,
+    theory W    <- WB,
+    theory WE   <- WBE.
+
+  clone include BS_WB_WS_U with
+        op sizeS <- sizeS,
+        op sizeB <- sizeB,
+    theory WS    <- WS,
+    theory WSE   <- WSE,
+    theory WB    <- WB,
+    theory WBE   <- WBE,
+    theory BSWS  <- BSWS,
+    theory BSWB  <- BSWB,
+        op truncateu'S <- W_WS.truncateu'S,
+        op zeroextu'B  <- W_WS.zeroextu'B,
+        op sigextu'B   <- W_WS.sigextu'B
+    rename [theory] "WS" as "WS_"
+           [theory] "WB" as "WB_"
+    proof *.
+
+    realize le_size by smt(WS.gt0_size W_WS.gt0_r W_WS.sizeBrS).
+
+  bind op [WB.t & WS.t] (\bits'S) "aextract".
+
+  realize dvd_size by apply: size_div.
+
+  realize bvaextractP.
+  proof.
+  have ? := WS.gt0_size.
+  move=> bv base [#] ? lt; rewrite ltz_divRL in lt.
+  - by apply: WS.gt0_size. - by apply: dvd_size.
+  apply/eq_sym/(eq_from_nth false).
+  - rewrite size_take_condle // size_drop 1:/#.
+    rewrite !size_w2bits lez_maxr 1:/#.
+    by rewrite ifT // #smt:(dvd_size).
+  move=> i; rewrite size_w2bits => ?.
+  rewrite get_w2bits bits'SiE // nth_take ~-1://#.
+  by rewrite nth_drop //#.
+  qed.
+end BS_WB_WS.
+
+(* ==================================================================== *)
+abstract theory BSA.
+  op size : int.
+
+  axiom gt0_size : 0 < size.
+ 
+  clone import PolyArray as A with
+    op size <- size proof ge0_size by smt(gt0_size).
+
+  bind array A."_.[_]" A."_.[_<-_]" A.to_list A.of_list A.t size.
+
+  realize gt0_size by exact: gt0_size.
+  realize tolistP  by done.
+  realize get_setP by smt(A.get_setE).
+  realize eqP      by smt(A.tP).
+  realize get_out  by smt(A.get_out).
+  realize oflistP by smt(A.get_of_list).
+end BSA.
+
+(* ==================================================================== *)
+abstract theory BSWA.
+  op asize : int.
+  op bsize : int.
+
+  clone import PolyArray as A with op size <- asize.
+  clone import BitWord   as W with op size <- bsize.
+
+  clone WE with
+        op size <- bsize,
+    theory W    <- W.
+
+  clone import BSBW as BSW with 
+        op size <- bsize,
+    theory BW   <- W,
+    theory WE   <- WE.
+
+   clone import BSA with
+        op size <- asize,
+    theory  A   <- A.
+
+  op init (f: int -> W.t) : W.t A.t = A.init f.
+
+  bind op [W.t & A.t] init "ainit".
+
+  realize bvainitP.
+  proof.
+  move=> f @/init; rewrite BVA_Top_BSA_A_t.tolistP.
+  by apply: eq_in_mkseq => i ? /=; rewrite initE ifT.
+  qed.
+end BSWA.
+
+(* ==================================================================== *)
+abstract theory BSWAS.
+  op asize : int.
+  op bsize : int.
+  op ssize : int.
+
+  axiom le_size : ssize <= bsize * asize.
+
+  clone import PolyArray as A  with op size <- asize.
+  clone import BitWord   as WB with op size <- bsize.
+  clone import BitWord   as WS with op size <- ssize.
+
+  clone WE as WEB with
+        op size <- bsize,
+    theory W    <- WB.
+
+  clone import BSBW as BSWB with 
+        op size <- bsize,
+    theory BW   <- WB,
+    theory WE   <- WEB.
+
+  clone WE as WES with
+        op size <- ssize,
+    theory W    <- WS.
+
+  clone import BSBW as BSWS with 
+        op size <- ssize,
+    theory BW   <- WS,
+    theory WE   <- WES.
+
+  clone BSA with
+        op size <- asize,
+    theory A    <- A.
+
+  clone BSWA with
+        op asize <- asize,
+        op bsize <- bsize,
+    theory W     <- WB,
+    theory WE    <- WEB,
+    theory BSW   <- BSWB,
+    theory A     <- A,
+    theory BSA   <- BSA.
+
+  op tobits (a : WB.t A.t) : bool list =
+    flatten (List.map WB.w2bits (A.to_list a)).
+
+  op ofbits (a : bool list) : WB.t A.t =
+    A.of_list witness (List.map WB.bits2w (chunk bsize a)).
+
+  lemma size_tobits a : size (tobits a) = bsize * asize.
+  proof.
+  rewrite /tobits (size_flatten_ctt bsize).
+  - by move=> bs /mapP[w] [_ ->].
+  - by rewrite size_map size_to_list.
+  qed.
+
+  hint simplify size_tobits.
+
+  lemma ofbitsK (bs : bool list) :
+    size bs = bsize * asize => tobits (ofbits bs) = bs.
+  proof.
+  move=> eq @/tobits @/ofbits; rewrite of_listK.
+  - by rewrite size_map size_chunk // eq; smt(WB.gt0_size).
+  rewrite -map_comp -(iffLR _ _ (eq_in_map idfun _ _)).
+  - move=> w /(in_chunk_size bsize _ _ WB.gt0_size) ?.
+    by rewrite /idfun /(\o) WB.bits2wK.
+  by rewrite map_id chunkK // eq dvdz_mulr dvdzz.
+  qed.
+
+  op sliceget (a : WB.t A.t) (offset : int) : WS.t =
+    WS.bits2w (take ssize (drop offset (tobits a))).
+
+  op sliceset (a : WB.t A.t) (offset : int) (w : WS.t) : WB.t A.t =
+    let pr = take offset (tobits a) in
+    let po = drop (offset + ssize) (tobits a) in
+    ofbits (pr ++ WS.w2bits w ++ po).
+
+  bind op [WB.t & WS.t & A.t] sliceget "asliceget".
+
+  realize le_size by exact: le_size.
+
+  realize bvaslicegetP.
+  proof. by move=> /= a off ? i ? @/sliceget; rewrite get_bits2w. qed.
+
+  bind op [WB.t & WS.t & A.t] sliceset "asliceset".
+
+  realize le_size by exact: le_size.
+
+  realize bvaslicesetP.
+  proof.
+  have ? := WS.ge0_size; have ? := WB.ge0_size.
+  move=> /= a off w ? i ?; rewrite -!/(tobits _) /sliceset /= ofbitsK.
+  - by rewrite !size_cat /= size_take_condle 1:/# /= ifT 1:/# size_drop /#.
+  case: (i < off) => ?.
+  - rewrite ifF 1:/# -catA nth_cat ifT.
+    - by rewrite size_take_condle /#.
+    - by rewrite nth_take ~-1:/#.
+  rewrite -catA nth_cat ifF 1:size_take_condle ~-1:/#.
+  rewrite size_take_condle 1:/# /= ifT 1:/# /=.
+  case: (off + ssize <= i) => ?.
+  - by rewrite ifF 1:/# nth_cat /= ifF 1:/# nth_drop /#.
+  by rewrite ifT 1:/# nth_cat ifT 1:/# get_w2bits.
+  qed.
+end BSWAS.
+
+(* ==================================================================== *)
+clone BSW as BSW16 with
+  op     size <- 16,
+  theory W    <- W16  { rename "_XX" as "_16" },
+  theory WE   <- WE16.
+
+(* -------------------------------------------------------------------- *)
+clone BSW as BSW32 with
+  op     size <- 32,
+  theory W    <- W32  { rename "_XX" as "_32" },
+  theory WE   <- WE32.
+
+(* -------------------------------------------------------------------- *)
+clone BSW as BSW64 with
+  op     size <- 64,
+  theory W    <- W64  { rename "_XX" as "_64" },
+  theory WE   <- WE64.
+
+(* -------------------------------------------------------------------- *)
+clone BSW as BSW128 with
+  op     size <- 128,
+  theory W    <- W128  { rename "_XX" as "_128" },
+  theory WE   <- WE128.
+
+(* -------------------------------------------------------------------- *)
+clone BSW as BSW256 with
+  op     size <- 256,
+  theory W    <- W256  { rename "_XX" as "_256" },
+  theory WE   <- WE256.
+
+(* ==================================================================== *)
+clone BS_WB_WS as BS_W2u16 with
+      op sizeS <-  16,
+      op sizeB <-  32,
+      op r     <-   2,
+  theory WS    <- W16   { rename "_XX" as "_16" },
+  theory WB    <- W32   { rename "_XX" as "_32" },
+  theory WSE   <- WE16,
+  theory WBE   <- WE32,
+  theory BSWS  <- BSW16,
+  theory BSWB  <- BSW32,
+  theory W_WS  <- W2u16
+                    { rename "'Ru'S" as "2u16"
+                             "'R"    as "2"
+                             "'S"    as "16"
+                             "'B"    as "32" }.
+
+(* -------------------------------------------------------------------- *)
+clone BS_WB_WS as BS_W2u32 with
+      op sizeS <-  32,
+      op sizeB <-  64,
+      op r     <-   2,
+  theory WS    <- W32   { rename "_XX" as "_32" },
+  theory WB    <- W64   { rename "_XX" as "_64" },
+  theory WSE   <- WE32,
+  theory WBE   <- WE64,
+  theory BSWS  <- BSW32,
+  theory BSWB  <- BSW64,
+  theory W_WS  <- W2u32
+                    { rename "'Ru'S" as "2u32"
+                             "'R"    as "2"
+                             "'S"    as "32"
+                             "'B"    as "64" }.
+
+(* -------------------------------------------------------------------- *)
+clone BS_WB_WS as BS_W2u64 with
+      op sizeS <-  64,
+      op sizeB <- 128,
+      op r     <-   2,
+  theory WS    <- W64   { rename "_XX" as "_64" },
+  theory WB    <- W128  { rename "_XX" as "_128" },
+  theory WSE   <- WE64,
+  theory WBE   <- WE128,
+  theory BSWS  <- BSW64,
+  theory BSWB  <- BSW128,
+  theory W_WS  <- W2u64
+                    { rename "'Ru'S" as "2u64"
+                             "'R"    as "2"
+                             "'S"    as "64"
+                             "'B"    as "128" }.
+
+(* -------------------------------------------------------------------- *)
+clone BS_WB_WS as BS_W2u128 with
+      op sizeS <- 128,
+      op sizeB <- 256,
+      op r     <-   2,
+  theory WS    <- W128  { rename "_XX" as "_128" },
+  theory WB    <- W256  { rename "_XX" as "_256" },
+  theory WSE   <- WE128,
+  theory WBE   <- WE256,
+  theory BSWS  <- BSW128,
+  theory BSWB  <- BSW256,
+  theory W_WS  <- W2u128
+                    { rename "'Ru'S" as "2u128"
+                             "'R"    as "2"
+                             "'S"    as "128"
+                             "'B"    as "256" }.
+
+(* -------------------------------------------------------------------- *)
+clone BS_WB_WS as BS_W4u16 with
+      op sizeS <-  16,
+      op sizeB <-  64,
+      op r     <-   4,
+  theory WS    <- W16   { rename "_XX" as "_16" },
+  theory WB    <- W64   { rename "_XX" as "_64" },
+  theory WSE   <- WE16,
+  theory WBE   <- WE64,
+  theory BSWS  <- BSW16,
+  theory BSWB  <- BSW64,
+  theory W_WS  <- W4u16
+                    { rename "'Ru'S" as "4u16"
+                             "'R"    as "4"
+                             "'S"    as "16"
+                             "'B"    as "64" }.
+
+(* -------------------------------------------------------------------- *)
+clone BS_WB_WS as BS_W4u32 with
+      op sizeS <-  32,
+      op sizeB <- 128,
+      op r     <-   4,
+  theory WS    <- W32   { rename "_XX" as "_32" },
+  theory WB    <- W128  { rename "_XX" as "_128" },
+  theory WSE   <- WE32,
+  theory WBE   <- WE128,
+  theory BSWS  <- BSW32,
+  theory BSWB  <- BSW128,
+  theory W_WS  <- W4u32
+                    { rename "'Ru'S" as "4u32"
+                             "'R"    as "4"
+                             "'S"    as "32"
+                             "'B"    as "128" }.
+
+(* -------------------------------------------------------------------- *)
+clone BS_WB_WS as BS_W4u64 with
+      op sizeS <-  64,
+      op sizeB <- 256,
+      op r     <-   4,
+  theory WS    <- W64   { rename "_XX" as "_64" },
+  theory WB    <- W256  { rename "_XX" as "_256" },
+  theory WSE   <- WE64,
+  theory WBE   <- WE256,
+  theory BSWS  <- BSW64,
+  theory BSWB  <- BSW256,
+  theory W_WS  <- W4u64
+                    { rename "'Ru'S" as "4u64"
+                             "'R"    as "4"
+                             "'S"    as "64"
+                             "'B"    as "256" }.
+
+(* -------------------------------------------------------------------- *)
+clone BS_WB_WS as BS_W8u16 with
+      op sizeS <-  16,
+      op sizeB <- 128,
+      op r     <-   8,
+  theory WS    <- W16   { rename "_XX" as "_16" },
+  theory WB    <- W128  { rename "_XX" as "_128" },
+  theory WSE   <- WE16,
+  theory WBE   <- WE128,
+  theory BSWS  <- BSW16,
+  theory BSWB  <- BSW128,
+  theory W_WS  <- W8u16
+                    { rename "'Ru'S" as "8u16"
+                             "'R"    as "8"
+                             "'S"    as "16"
+                             "'B"    as "128" }.
+
+(* -------------------------------------------------------------------- *)
+clone BS_WB_WS as BS_W8u32 with
+      op sizeS <-  32,
+      op sizeB <- 256,
+      op r     <-   8,
+  theory WS    <- W32   { rename "_XX" as "_32" },
+  theory WB    <- W256  { rename "_XX" as "_256" },
+  theory WSE   <- WE32,
+  theory WBE   <- WE256,
+  theory BSWS  <- BSW32,
+  theory BSWB  <- BSW256,
+  theory W_WS  <- W8u32
+                    { rename "'Ru'S" as "8u32"
+                             "'R"    as "8"
+                             "'S"    as "32"
+                             "'B"    as "256" }.
+
+(* -------------------------------------------------------------------- *)
+clone BS_WB_WS as BS_W16u16 with
+      op sizeS <-  16,
+      op sizeB <- 256,
+      op r     <-  16,
+  theory WS    <- W16   { rename "_XX" as "_16" },
+  theory WB    <- W256  { rename "_XX" as "_256" },
+  theory WSE   <- WE16,
+  theory WBE   <- WE256,
+  theory BSWS  <- BSW16,
+  theory BSWB  <- BSW256,
+  theory W_WS  <- W16u16
+                    { rename "'Ru'S" as "16u16"
+                             "'R"    as "16"
+                             "'S"    as "16"
+                             "'B"    as "256" }.
+
