proof/eclib/List_extra.ec
@@ -105,3 +105,44 @@ lemma all_range_2_eq P Q (min1 max1 min2 max2 : int) :
   all_range_2 P min1 max1 min2 max2 <=>
   all_range_2 Q min1 max1 min2 max2.
 proof. by move => Heq2; apply all_range_eq => y Hy_range /=; apply all_range_eq => x Hx_range /=; apply Heq2. qed.
+
+(* ==================================================================== *)
+(* Generic list lemmas consumed by CircuitBindings (ported from mldsa   *)
+(* ListExtra.ec).                                                        *)
+(* ==================================================================== *)
+
+lemma in_map_id ['a] (f : 'a -> 'a) (s : 'a list) :
+  (forall x, x \in s => f x = x) => map f s = s.
+proof. by move=> id_f; rewrite -{2}[s]map_id &(eq_in_map). qed.
+
+lemma in_map_cancel ['a 'b] (f : 'a -> 'b) (g : 'b -> 'a) (s : 'a list) :
+  (forall x, x \in s => g (f x) = x) => map g (map f s) = s.
+proof. by move=> can_fg; rewrite -map_comp in_map_id. qed.
+
+lemma flatten_map_seq1 ['a 'b] (f : 'a -> 'b) (s : 'a list) :
+  flatten (map (fun x => [f x]) s) = map f s.
+proof. by elim: s. qed.
+
+lemma flatten_mkseq_seq1 ['a] (f : int -> 'a) (n : int) :
+  flatten (mkseq (fun i => [f i]) n) = mkseq f n.
+proof. by apply: flatten_map_seq1. qed.
+
+(* -------------------------------------------------------------------- *)
+lemma take_mkseqE ['a] (x0 : 'a) (s : 'a list) (i : int) : 0 <= i <= size s =>
+  take i s = mkseq (fun j => nth x0 s j) i.
+proof.
+move=> ?; apply/eq_sym/(eq_from_nth x0).
+- by rewrite size_take ~-1:/# size_mkseq /#.
+rewrite size_mkseq lez_maxr 1:/# => j rgj.
+by rewrite nth_mkseq //= nth_take //#.
+qed.
+
+(* -------------------------------------------------------------------- *)
+lemma drop_mkseqE ['a] (x0 : 'a) (s : 'a list) (i : int) : 0 <= i <= size s =>
+  drop i s = mkseq (fun j => nth x0 s (i + j)) (size s - i).
+proof.
+move=> ?; apply/eq_sym/(eq_from_nth x0).
+- by rewrite size_drop ~-1:/# size_mkseq /#.
+rewrite size_mkseq lez_maxr 1:/# => j rgj.
+by rewrite nth_mkseq //= nth_drop //#.
+qed.
