proof/xarrays/XArray1024.ec
@@ -1,0 +1,117 @@
+(* -------------------------------------------------------------------- *)
+require import AllCore List IntDiv JWordExtra CircuitBindings.
+from JazzEC require import Array1024.
+require import XWord11 XWord12.
+
+from Jasmin require import JWord.
+
+(* -------------------------------------------------------------------- *)
+export Array1024.
+
+(* -------------------------------------------------------------------- *)
+clone export PAE with
+      op size <- 1024,
+  theory A    <- Array1024.
+
+(* -------------------------------------------------------------------- *)
+clone BSA as BSA1024 with
+      op size <- 1024,
+  theory A    <- Array1024
+
+  proof gt0_size by done.
+
+(* -------------------------------------------------------------------- *)
+clone BSWA as BSWA_1024u16 with
+      op asize <- 1024,
+      op bsize <- 16,
+  theory A     <- Array1024,
+  theory BSA   <- BSA1024,
+  theory W     <- W16 { rename "_XX" as "_16" },
+  theory WE    <- WE16,
+  theory BSW   <- BSW16.
+
+(* -------------------------------------------------------------------- *)
+clone BSWA as BSWA_1024u12 with
+      op asize <- 1024,
+      op bsize <- 12,
+  theory A     <- Array1024,
+  theory BSA   <- BSA1024,
+  theory W     <- W12 { rename "_XX" as "_12" },
+  theory WE    <- WE12,
+  theory BSW   <- BSW12.
+
+(* -------------------------------------------------------------------- *)
+clone BSWA as BSWA_1024u11 with
+      op asize <- 1024,
+      op bsize <- 11,
+  theory A     <- Array1024,
+  theory BSA   <- BSA1024,
+  theory W     <- W11 { rename "_XX" as "_11" },
+  theory WE    <- WE11,
+  theory BSW   <- BSW11.
+
+(* -------------------------------------------------------------------- *)
+clone BSWA as BSWA_1024u8 with
+      op asize <- 1024,
+      op bsize <- 8,
+  theory A     <- Array1024,
+  theory BSA   <- BSA1024,
+  theory W     <- W8 { rename "_XX" as "_8" },
+  theory WE    <- WE8,
+  theory BSW   <- BSW8
+  proof *.
+
+(* -------------------------------------------------------------------- *)
+clone BSWAS as BSWAS_1024u16_256 with
+      op asize   <- 1024,
+      op bsize   <- 16,
+      op ssize   <- 256,
+  theory A       <- Array1024,
+  theory BSA     <- BSA1024,
+  theory WB      <- W16  { rename "_XX" as "_16" },
+  theory WEB     <- WE16,
+  theory BSWB    <- BSW16,
+  theory WS      <- W256  { rename "_XX" as "_256" },
+  theory WES     <- WE256,
+  theory BSWS    <- BSW256,
+  theory BSWA    <- BSWA_1024u16
+
+  proof le_size by done.
+
+from JazzEC require import WArray2048.
+require import BitEncoding.
+import Array1024 BitChunking.
+
+lemma BSWAS_1024u16_256_slicegetE o (p : W16.t Array1024.t):
+    0 <= o*8 <= 1024*16-256 =>
+     get256_direct (WArray2048.init16 (fun (i_0 : int) => p.[i_0])) o = BSWAS_1024u16_256.sliceget p (o * 8).
+  proof.
+  move => Ho.
+  rewrite /get256_direct /pack32_t;apply W256.wordP => k kb.
+  have //= := BSWAS_1024u16_256.BVA_asliceget_Top_CircuitBindings_BSWAS_WB_t_Top_CircuitBindings_BSWAS_WS_t_Top_CircuitBindings_BSWAS_A_t.bvaslicegetP p (o * 8) _; 1: by smt().
+  move => -> //; rewrite initiE 1:/# /= initiE 1:/# /= initiE 1:/# /= /(\bits8) initiE 1:/# /=.
+  rewrite nth_take 1,2:/# nth_drop 1,2:/#  (nth_flatten false 16).
+  + rewrite allP /= => x; rewrite mapP => He; elim He;smt(W16.size_w2bits).
+  rewrite (nth_map witness); 1: by rewrite size_to_list; smt().
+  by rewrite get_to_list get_w2bits /#.
+ qed.
+
+lemma BSWAS_1024u16_256_slicesetE (t : W16.t Array1024.t) o (s : W256.t) :
+  0 <= (o*8) <= 16 * 1024 - 256 =>
+   BSWAS_1024u16_256.sliceset t (o*8) s =
+      Array1024.init (get16 (set256_direct (WArray2048.init16 (fun (i_0 : int) => t.[i_0])) o s)).
+proof.
+move => Ho.
+rewrite tP => k kb.
+rewrite wordP => i ib;rewrite initiE 1:/# /=.
+have //= := BSWAS_1024u16_256.BVA_asliceset_Top_CircuitBindings_BSWAS_WB_t_Top_CircuitBindings_BSWAS_WS_t_Top_CircuitBindings_BSWAS_A_t.bvaslicesetP t (o*8) s _ (k*16+i) _;1,2:by smt().
+rewrite (nth_flatten false 16).
++ rewrite allP /= => x; rewrite mapP => He; elim He;smt(W16.size_w2bits).
+rewrite (nth_map witness); 1: by rewrite size_to_list; smt().
+rewrite get_to_list get_w2bits (: (k * 16 + i) %/ 16 = k) 1:/# (: (k * 16 + i) %% 16 = i) 1:/# => -> .
+rewrite (nth_flatten false 16).
++ rewrite allP /= => x; rewrite mapP => He; elim He;smt(W16.size_w2bits).
+rewrite (nth_map witness); 1: by rewrite size_to_list; smt().
+rewrite get_w2bits get_to_list get16E pack2E initiE 1:/# /= /set256_direct initiE 1:/# /= /(\bits8) initiE 1:/# /= /init16 initiE 1:/# /=.
+by smt(W8.initiE).
+qed.
