proof/xarrays/XArray128.ec
@@ -1,0 +1,110 @@
+(* -------------------------------------------------------------------- *)
+require import AllCore List IntDiv JWordExtra CircuitBindings.
+from JazzEC require import Array128.
+
+from Jasmin require import JWord.
+
+(* -------------------------------------------------------------------- *)
+export Array128.
+
+(* -------------------------------------------------------------------- *)
+clone export PAE with
+      op size <- 128,
+  theory A    <- Array128.
+
+(* -------------------------------------------------------------------- *)
+clone BSA as BSA128 with
+      op size <- 128,
+  theory A    <- Array128
+
+  proof gt0_size by done.
+
+(* -------------------------------------------------------------------- *)
+clone BSWA as BSWA_128u8 with
+      op asize <- 128,
+      op bsize <- 8,
+  theory A     <- Array128,
+  theory BSA   <- BSA128,
+  theory W     <- W8 { rename "_XX" as "_8" },
+  theory WE    <- WE8,
+  theory BSW   <- BSW8
+  proof *.
+
+(* -------------------------------------------------------------------- *)
+clone BSWAS as BSWAS_128u8_256 with
+      op asize   <- 128, op bsize <- 8, op ssize <- 256,
+  theory A    <- Array128, theory BSA <- BSA128,
+  theory WB   <- W8  { rename "_XX" as "_8" },  theory WEB <- WE8,  theory BSWB <- BSW8,
+  theory WS   <- W256 { rename "_XX" as "_256" }, theory WES <- WE256, theory BSWS <- BSW256,
+  theory BSWA <- BSWA_128u8
+  proof le_size by done.
+
+(* -------------------------------------------------------------------- *)
+clone BSWAS as BSWAS_128u8_64 with
+      op asize   <- 128, op bsize <- 8, op ssize <- 64,
+  theory A    <- Array128, theory BSA <- BSA128,
+  theory WB   <- W8  { rename "_XX" as "_8" }, theory WEB <- WE8, theory BSWB <- BSW8,
+  theory WS   <- W64 { rename "_XX" as "_64" }, theory WES <- WE64, theory BSWS <- BSW64,
+  theory BSWA <- BSWA_128u8
+  proof le_size by done.
+
+(* -------------------------------------------------------------------- *)
+clone BSWAS as BSWAS_128u8_16 with
+      op asize   <- 128, op bsize <- 8, op ssize <- 16,
+  theory A    <- Array128, theory BSA <- BSA128,
+  theory WB   <- W8  { rename "_XX" as "_8" }, theory WEB <- WE8, theory BSWB <- BSW8,
+  theory WS   <- W16 { rename "_XX" as "_16" }, theory WES <- WE16, theory BSWS <- BSW16,
+  theory BSWA <- BSWA_128u8
+  proof le_size by done.
+
+from JazzEC require import WArray128.
+require import BitEncoding.
+import Array128 BitChunking.
+
+lemma BSWAS_128u8_64_slicegetE o (p : W8.t Array128.t):
+    0 <= o*8 <= 128*8-64 =>
+     get64_direct (WArray128.init8 (fun (i_0 : int) => p.[i_0])) o = BSWAS_128u8_64.sliceget p (o * 8).
+  proof.
+  move => Ho.
+  rewrite /get64_direct /pack8_t;apply W64.wordP => k kb.
+  have //= := BSWAS_128u8_64.BVA_asliceget_Top_CircuitBindings_BSWAS_WB_t_Top_CircuitBindings_BSWAS_WS_t_Top_CircuitBindings_BSWAS_A_t.bvaslicegetP p (o * 8) _; 1: by smt().
+  move => -> //; rewrite initiE 1:/# /= initiE 1:/# /= initiE 1:/# /=.
+  rewrite nth_take 1,2:/# nth_drop 1,2:/#  (nth_flatten false 8).
+  + rewrite allP /= => x; rewrite mapP => He; elim He;smt(W8.size_w2bits).
+  rewrite (nth_map witness); 1: by rewrite size_to_list; smt().
+  by rewrite get_to_list get_w2bits /#.
+ qed.
+
+lemma BSWAS_128u8_16_slicegetE o (p : W8.t Array128.t):
+    0 <= o*8 <= 128*8-16 =>
+     get16_direct (WArray128.init8 (fun (i_0 : int) => p.[i_0])) o = BSWAS_128u8_16.sliceget p (o * 8).
+  proof.
+  move => Ho.
+  rewrite /get16_direct /pack2_t;apply W16.wordP => k kb.
+  have //= := BSWAS_128u8_16.BVA_asliceget_Top_CircuitBindings_BSWAS_WB_t_Top_CircuitBindings_BSWAS_WS_t_Top_CircuitBindings_BSWAS_A_t.bvaslicegetP p (o * 8) _; 1: by smt().
+  move => -> //; rewrite initiE 1:/# /= initiE 1:/# /= initiE 1:/# /=.
+  rewrite nth_take 1,2:/# nth_drop 1,2:/#  (nth_flatten false 8).
+  + rewrite allP /= => x; rewrite mapP => He; elim He;smt(W8.size_w2bits).
+  rewrite (nth_map witness); 1: by rewrite size_to_list; smt().
+  by rewrite get_to_list get_w2bits /#.
+ qed.
+
+lemma BSWAS_128u8_256_slicesetE (t : W8.t Array128.t) o (s : W256.t) :
+  0 <= (o*8) <= 8 * 128 - 256 =>
+   BSWAS_128u8_256.sliceset t (o*8) s =
+      Array128.init (get8 (set256_direct (WArray128.init8 (fun (i_0 : int) => t.[i_0])) o s)).
+proof.
+move => Ho.
+rewrite tP => k kb.
+rewrite wordP => i ib;rewrite initiE 1:/# /=.
+have //= := BSWAS_128u8_256.BVA_asliceset_Top_CircuitBindings_BSWAS_WB_t_Top_CircuitBindings_BSWAS_WS_t_Top_CircuitBindings_BSWAS_A_t.bvaslicesetP t (o*8) s _ (k*8+i) _;1,2:by smt().
+rewrite (nth_flatten false 8).
++ rewrite allP /= => x; rewrite mapP => He; elim He;smt(W8.size_w2bits).
+rewrite (nth_map witness); 1: by rewrite size_to_list; smt().
+rewrite get_to_list get_w2bits (: (k * 8 + i) %/ 8 = k) 1:/# (: (k * 8 + i) %% 8 = i) 1:/# => -> .
+rewrite (nth_flatten false 8).
++ rewrite allP /= => x; rewrite mapP => He; elim He;smt(W8.size_w2bits).
+rewrite (nth_map witness); 1: by rewrite size_to_list; smt().
+rewrite get_w2bits get_to_list /get8 /set256_direct initiE 1:/# /= /(\bits8) initiE 1:/# /=.
+by smt(W8.initiE).
+qed.
