proof/xarrays/XArray1536.ec
@@ -1,0 +1,31 @@
+(* -------------------------------------------------------------------- *)
+require import AllCore List IntDiv JWordExtra CircuitBindings.
+from JazzEC require import Array1536.
+
+from Jasmin require import JWord.
+
+(* -------------------------------------------------------------------- *)
+export Array1536.
+
+(* -------------------------------------------------------------------- *)
+clone export PAE with
+      op size <- 1536,
+  theory A    <- Array1536.
+
+(* -------------------------------------------------------------------- *)
+clone BSA as BSA1536 with
+      op size <- 1536,
+  theory A    <- Array1536
+
+  proof gt0_size by done.
+
+(* -------------------------------------------------------------------- *)
+clone BSWA as BSWA_1536u8 with
+      op asize <- 1536,
+      op bsize <- 8,
+  theory A     <- Array1536,
+  theory BSA   <- BSA1536,
+  theory W     <- W8 { rename "_XX" as "_8" },
+  theory WE    <- WE8,
+  theory BSW   <- BSW8
+  proof *.
