proof/xarrays/XArray16.ec
@@ -1,0 +1,107 @@
+(* -------------------------------------------------------------------- *)
+require import AllCore List IntDiv JWordExtra CircuitBindings.
+from JazzEC require import Array16.
+
+from Jasmin require import JWord.
+
+(* -------------------------------------------------------------------- *)
+export Array16.
+
+(* -------------------------------------------------------------------- *)
+clone export PAE with
+      op size <- 16,
+  theory A    <- Array16.
+
+(* -------------------------------------------------------------------- *)
+clone BSA as BSA16 with
+      op size <- 16,
+  theory A    <- Array16
+
+  proof gt0_size by done.
+
+(* -------------------------------------------------------------------- *)
+clone BSWA as BSWA_16u16 with
+      op asize <- 16,
+      op bsize <- 16,
+  theory A     <- Array16,
+  theory BSA   <- BSA16,
+  theory W     <- W16 { rename "_XX" as "_16" },
+  theory WE    <- WE16,
+  theory BSW   <- BSW16.
+
+(* -------------------------------------------------------------------- *)
+clone BSWAS as BSWAS_16u16_256 with
+      op asize   <- 16,
+      op bsize   <- 16,
+      op ssize   <- 256,
+  theory A       <- Array16,
+  theory BSA     <- BSA16,
+  theory WB      <- W16  { rename "_XX" as "_16" },
+  theory WEB     <- WE16,
+  theory BSWB    <- BSW16,
+  theory WS      <- W256  { rename "_XX" as "_256" },
+  theory WES     <- WE256,
+  theory BSWS    <- BSW256,
+  theory BSWA    <- BSWA_16u16
+
+  proof le_size by done.
+
+(* -------------------------------------------------------------------- *)
+clone BSWA as BSWA_16u8 with
+      op asize <- 16,
+      op bsize <- 8,
+  theory A     <- Array16,
+  theory BSA   <- BSA16,
+  theory W     <- W8 { rename "_XX" as "_8" },
+  theory WE    <- WE8,
+  theory BSW   <- BSW8
+  proof *.
+
+(* -------------------------------------------------------------------- *)
+clone BSWAS as BSWAS_16u8_128 with
+      op asize   <- 16,
+      op bsize   <- 8,
+      op ssize   <- 128,
+  theory A       <- Array16,
+  theory BSA     <- BSA16,
+  theory WB      <- W8  { rename "_XX" as "_8" },
+  theory WEB     <- WE8,
+  theory BSWB    <- BSW8,
+  theory WS      <- W128  { rename "_XX" as "_128" },
+  theory WES     <- WE128,
+  theory BSWS    <- BSW128,
+  theory BSWA    <- BSWA_16u8
+
+  proof le_size by done.
+
+from JazzEC require import WArray16 WArray32.
+require import BitEncoding.
+import Array16 BitChunking.
+
+lemma BSWAS_16u16_256_slicegetE o (p : W16.t Array16.t):
+    0 <= o*8 <= 16*16-256 =>
+     get256_direct (WArray32.init16 (fun (i_0 : int) => p.[i_0])) o = BSWAS_16u16_256.sliceget p (o * 8).
+  proof.
+  move => Ho.
+  rewrite /get256_direct /pack32_t;apply W256.wordP => k kb.
+  have //= := BSWAS_16u16_256.BVA_asliceget_Top_CircuitBindings_BSWAS_WB_t_Top_CircuitBindings_BSWAS_WS_t_Top_CircuitBindings_BSWAS_A_t.bvaslicegetP p (o * 8) _; 1: by smt().
+  move => -> //; rewrite initiE 1:/# /= initiE 1:/# /= initiE 1:/# /= /(\bits8) initiE 1:/# /=.
+  rewrite nth_take 1,2:/# nth_drop 1,2:/#  (nth_flatten false 16).
+  + rewrite allP /= => x; rewrite mapP => He; elim He;smt(W16.size_w2bits).
+  rewrite (nth_map witness); 1: by rewrite size_to_list; smt().
+  by rewrite get_to_list get_w2bits /#.
+ qed.
+
+lemma BSWAS_16u8_128_slicegetE o (p : W8.t Array16.t):
+    0 <= o*8 <= 16*8-128 =>
+     get128_direct (WArray16.init8 (fun (i_0 : int) => p.[i_0])) o = BSWAS_16u8_128.sliceget p (o * 8).
+  proof.
+  move => Ho.
+  rewrite /get128_direct /pack16_t;apply W128.wordP => k kb.
+  have //= := BSWAS_16u8_128.BVA_asliceget_Top_CircuitBindings_BSWAS_WB_t_Top_CircuitBindings_BSWAS_WS_t_Top_CircuitBindings_BSWAS_A_t.bvaslicegetP p (o * 8) _; 1: by smt().
+  move => -> //; rewrite initiE 1:/# /= initiE 1:/# /= initiE 1:/# /=.
+  rewrite nth_take 1,2:/# nth_drop 1,2:/#  (nth_flatten false 8).
+  + rewrite allP /= => x; rewrite mapP => He; elim He;smt(W8.size_w2bits).
+  rewrite (nth_map witness); 1: by rewrite size_to_list; smt().
+  by rewrite get_to_list get_w2bits /#.
+ qed.
