proof/xarrays/XArray24.ec
@@ -1,0 +1,31 @@
+(* -------------------------------------------------------------------- *)
+require import AllCore List IntDiv JWordExtra CircuitBindings XWord12.
+from JazzEC require import Array24.
+
+from Jasmin require import JWord.
+
+(* -------------------------------------------------------------------- *)
+export Array24.
+
+(* -------------------------------------------------------------------- *)
+clone export PAE with
+      op size <- 24,
+  theory A    <- Array24.
+
+(* -------------------------------------------------------------------- *)
+clone BSA as BSA24 with
+      op size <- 24,
+  theory A    <- Array24
+
+  proof gt0_size by done.
+
+(* -------------------------------------------------------------------- *)
+clone BSWA as BSWA_24u8 with
+      op asize <- 24,
+      op bsize <- 8,
+  theory A     <- Array24,
+  theory BSA   <- BSA24,
+  theory W     <- W8 { rename "_XX" as "_8" },
+  theory WE    <- WE8,
+  theory BSW   <- BSW8
+  proof *.
