proof/xarrays/XArray25.ec
@@ -1,0 +1,30 @@
+(* -------------------------------------------------------------------- *)
+require import AllCore List IntDiv JWordExtra CircuitBindings.
+from JazzEC require import Array25.
+
+from Jasmin require import JWord.
+
+(* -------------------------------------------------------------------- *)
+export Array25.
+
+(* -------------------------------------------------------------------- *)
+clone export PAE with
+      op size <- 25,
+  theory A    <- Array25.
+
+(* -------------------------------------------------------------------- *)
+clone BSA as BSA25 with
+      op size <- 25,
+  theory A    <- Array25
+
+  proof gt0_size by done.
+
+(* -------------------------------------------------------------------- *)
+clone BSWA as BSWA_25u64 with
+      op asize <- 25,
+      op bsize <- 64,
+  theory A     <- Array25,
+  theory BSA   <- BSA25,
+  theory W     <- W64 { rename "_XX" as "_64" },
+  theory WE    <- WE64,
+  theory BSW   <- BSW64.
