proof/xarrays/XArray40.ec
@@ -1,0 +1,30 @@
+(* -------------------------------------------------------------------- *)
+require import AllCore List IntDiv JWordExtra CircuitBindings.
+from JazzEC require import Array40.
+
+from Jasmin require import JWord.
+
+(* -------------------------------------------------------------------- *)
+export Array40.
+
+(* -------------------------------------------------------------------- *)
+clone export PAE with
+      op size <- 40,
+  theory A    <- Array40.
+
+(* -------------------------------------------------------------------- *)
+clone BSA as BSA40 with
+      op size <- 40,
+  theory A    <- Array40
+  proof gt0_size by done.
+
+(* -------------------------------------------------------------------- *)
+clone BSWA as BSWA_40u16 with
+      op asize <- 40,
+      op bsize <- 16,
+  theory A     <- Array40,
+  theory BSA   <- BSA40,
+  theory W     <- W16 { rename "_XX" as "_16" },
+  theory WE    <- WE16,
+  theory BSW   <- BSW16
+  proof *.
