proof/xarrays/XArray48.ec
@@ -1,0 +1,31 @@
+(* -------------------------------------------------------------------- *)
+require import AllCore List IntDiv JWordExtra CircuitBindings XWord12.
+from JazzEC require import Array48.
+
+from Jasmin require import JWord.
+
+(* -------------------------------------------------------------------- *)
+export Array48.
+
+(* -------------------------------------------------------------------- *)
+clone export PAE with
+      op size <- 48,
+  theory A    <- Array48.
+
+(* -------------------------------------------------------------------- *)
+clone BSA as BSA48 with
+      op size <- 48,
+  theory A    <- Array48
+
+  proof gt0_size by done.
+
+(* -------------------------------------------------------------------- *)
+clone BSWA as BSWA_48u8 with
+      op asize <- 48,
+      op bsize <- 8,
+  theory A     <- Array48,
+  theory BSA   <- BSA48,
+  theory W     <- W8 { rename "_XX" as "_8" },
+  theory WE    <- WE8,
+  theory BSW   <- BSW8
+  proof *.
