proof/xarrays/XArray7.ec
@@ -1,0 +1,30 @@
+(* -------------------------------------------------------------------- *)
+require import AllCore List IntDiv JWordExtra CircuitBindings.
+from JazzEC require import Array7.
+
+from Jasmin require import JWord.
+
+(* -------------------------------------------------------------------- *)
+export Array7.
+
+(* -------------------------------------------------------------------- *)
+clone export PAE with
+      op size <- 7,
+  theory A    <- Array7.
+
+(* -------------------------------------------------------------------- *)
+clone BSA as BSA7 with
+      op size <- 7,
+  theory A    <- Array7
+
+  proof gt0_size by done.
+
+(* -------------------------------------------------------------------- *)
+clone BSWA as BSWA_7u256 with
+      op asize <- 7,
+      op bsize <- 256,
+  theory A     <- Array7,
+  theory BSA   <- BSA7,
+  theory W     <- W256 { rename "_XX" as "_256" },
+  theory WE    <- WE256,
+  theory BSW   <- BSW256.
