proof/xwords/XWord4.ec
@@ -1,0 +1,38 @@
+(* -------------------------------------------------------------------- *)
+require import AllCore.
+
+(* -------------------------------------------------------------------- *)
+from Jasmin require import JWord.
+
+require import JWordExtra CircuitBindings.
+
+(* -------------------------------------------------------------------- *)
+clone export BitWordSH as W4 with
+    op size <- 4
+    rename "_XX" as "_4"
+    proof gt0_size by done,
+          size_le_256 by done.
+
+clone WE as WE4 with
+  op     size <- 4,
+  theory W    <- W4 { rename "_XX" as "_4" }.
+
+clone BSW as BSW4 with
+  op     size <- 4,
+  theory W    <- W4  { rename "_XX" as "_4" },
+  theory WE   <- WE4 { rename "_XX" as "_4" }.
+
+clone BS_WB_WS_U as BS_W32_W4_U with
+        op sizeS <- 4,
+        op sizeB <- 32,
+    theory WS    <- W4  { rename "_XX" as "_4" },
+    theory WSE   <- WE4,
+    theory WB    <- W32  { rename "_XX" as "_32" },
+    theory WBE   <- WE32,
+    theory BSWS  <- BSW4,
+    theory BSWB  <- BSW32
+
+    rename "'S" as "4"
+    rename "'B" as "32"
+
+    proof le_size by done, *.
